Costed exercise function.

ContractExamples/FStar/CallOption.fst
@@ -4,6 +4,7 @@ module V = Zen.Vector
 module A = Zen.Array
 module O = Zen.Option
 module OT = Zen.OptionT
+module E = Zen.Error
 module ET = Zen.ErrorT
 module U64 = FStar.UInt64
 module Crypto = Zen.Crypto
@@ -13,14 +14,27 @@ module U32 = FStar.UInt32
 open Zen.Base
 open Zen.Types
 open Zen.Cost
+open Zen.Merkle
 open Zen.Types.Serialized.Realized
 
 
 let numeraire: cost hash 3 = ret @ Zen.Util.hashFromBase64 "AAAAAAAAAAAAAAAAAAAAAAAAAAAAAAAAAAAAAAAAAAA="
 
+// "price" is the premium, in kalapas
 let price: U64.t = 100UL
 
+// strike in u64 is real strike * 1000, rounded down
+let strike: U64.t = 1000000UL
+
 let oracleHash: cost hash 3 = ret @ Zen.Util.hashFromBase64 "AAAAAAAAAAAAAAAAAAAAAAAAAAAAAAAAAAAAAAAAAAA="
+
+// No string -> byte arrays, yet. So 32 byte arrays to represent
+// the underlying, i.e. stuff like "AAPL", "MSFT", etc. To use:
+// take string, cast to byte array, pad to 32 bytes, base64 encode,
+// pass in here.
+// The example decodes to "AAPL", followed by 28 zero bytes.
+let underlyingSymbol = ret @ Zen.Util.hashFromBase64
+"QUFQTAAAAAAAAAAAAAAAAAAAAAAAAAAAAAAAAAAAAAA="
 
 type pointedOutput = outpoint * output
 
@@ -151,13 +165,19 @@ let decodeState #n iData =
       ret @ {tokensIssued=tk; collateral=coll; counter=cter}
     | _ -> autoFailw "Bad data"
 
-val createTx : hash -> command -> cost (result transactionSkeleton) 144
-let createTx cHash cmd =
-  do numeraire <-- numeraire;
-  let open ET in
-  let open U64 in
-  match cmd with
-  | Initialize (pt, oput) ->
+val findRoot : #n:nat -> inputData n -> (path:auditPath)
+    -> cost (result hash) M.((n * 384 + 1065 + dfst path.hashes))
+let findRoot #n iData {location=location;hashes=hashes} =
+  let inputHash = sha3_256 iData in
+  let optRoot = OT.bindLift inputHash (function h -> rootFromAuditPath h location (dsnd hashes)) in
+  do optRoot' <-- optRoot;
+  ret @ O.maybe (E.failw "Can't hash input data") (E.ret) optRoot'
+
+val initializeTx : hash -> pointedOutput -> cost (result transactionSkeleton) 45
+let initializeTx cHash (pt, oput) =
+      (do numeraire <-- numeraire;
+      let open ET in
+      let open U64 in
       if oput.spend.asset = numeraire
       then      // Initialize with data output
         let initialState : state =
@@ -166,27 +186,81 @@ let createTx cHash cmd =
             collateral=oput.spend.amount;
             counter=0UL;
           } in
-        do initialStateData <-- inc (retT @ encodeState initialState) 6;
+        do initialStateData <-- retT @ encodeState initialState;
         let dataOutputLock = ContractLock cHash 3 initialStateData in
         let dataOutput = {lock=dataOutputLock;spend=oput.spend} in
-        autoRet @ Tx [| pt |] [| dataOutput |] None
-      else autoFailw "Can't initialize with this asset."
-  | Collateralize [| (pt1,dataOutput); (pt2,newFundsOutput) |] ->
-    if dataOutput.spend.asset = numeraire && newFundsOutput.spend.asset = numeraire
-    then
-      begin match dataOutput.lock, newFundsOutput.lock with
+        ret @ Tx [| pt |] [| dataOutput |] None
+      else
+      autoFailw "Can't initialize with this asset.")
+
+
+val collateralizeTx :
+    hash
+    -> pointedOutput
+    -> pointedOutput
+    -> cost (result transactionSkeleton) 102
+let collateralizeTx cHash (pt1,dataOutput) (pt2,newFundsOutput) =
+      do numeraire <-- numeraire;
+      let open ET in
+      let open U64 in
+      if dataOutput.spend.asset = numeraire && newFundsOutput.spend.asset = numeraire
+      then
+        begin match dataOutput.lock, newFundsOutput.lock with
+        | ContractLock h1 3 currentStateData, ContractLock h2 _ _ ->
+            if h1 <> cHash || h2 <> cHash
+            then autoFailw "Locked to wrong contract"
+            else begin
+            do currentState <-- decodeState currentStateData;
+            // TODO: avoid modular addition!!
+            let newCollateral = currentState.collateral +%^ newFundsOutput.spend.amount in
+            let newState = {
+              tokensIssued = currentState.tokensIssued;
+              collateral = newCollateral;
+              counter = currentState.counter +%^ 1UL;   // We actually prefer modular arithmetic for the counter
+            } in
+            do newStateData <-- retT @ encodeState newState;
+            let newDataOutputLock = ContractLock cHash 3 newStateData in
+            let newDataOutput =
+              {
+                lock=newDataOutputLock;
+                spend={asset=numeraire;amount=newCollateral}
+              } in
+            ret @ Tx
+                    [| pt1; pt2 |]
+                    [| newDataOutput |]
+                    None
+            end
+        | _,_ -> autoFailw "Inputs not locked to this contract!"
+        end
+      else autoFailw "Can't use these asset types for Collateralize"
+
+
+val buyTx :
+    hash
+    -> pointedOutput
+    -> pointedOutput
+    -> outputLock
+    -> cost (result transactionSkeleton) 112
+let buyTx cHash (pt1, dataOutput) (pt2, purchaseOutput) lk =
+      do numeraire <-- numeraire;
+      let open ET in
+      let open U64 in
+      if dataOutput.spend.asset = numeraire && purchaseOutput.spend.asset = numeraire
+      then
+      begin match dataOutput.lock, purchaseOutput.lock with
       | ContractLock h1 3 currentStateData, ContractLock h2 _ _ ->
           if h1 <> cHash || h2 <> cHash
           then autoFailw "Locked to wrong contract"
           else begin
           do currentState <-- decodeState currentStateData;
           // TODO: avoid modular addition!!
-          let newCollateral = currentState.collateral +%^ newFundsOutput.spend.amount in
+          let newCollateral = currentState.collateral +%^ purchaseOutput.spend.amount in
+          let newTokens = purchaseOutput.spend.amount /^ price in   //downwards rounding
           let newState = {
-            tokensIssued = currentState.tokensIssued;
+            tokensIssued = currentState.tokensIssued +%^ newTokens; //TODO: modular
             collateral = newCollateral;
-            counter = currentState.counter +%^ 1UL;   // We actually prefer modular arithmetic for the counter
-          } in
+            counter = currentState.counter;
+          } in        //TODO: return to sender with insufficient collateral
           do newStateData <-- retT @ encodeState newState;
           let newDataOutputLock = ContractLock cHash 3 newStateData in
           let newDataOutput =
@@ -194,70 +268,126 @@ let createTx cHash cmd =
               lock=newDataOutputLock;
               spend={asset=numeraire;amount=newCollateral}
             } in
+          let buyersOutput =
+            {
+              lock=lk;
+              spend={asset=cHash;amount=newTokens}
+            } in
           ret @ Tx
                   [| pt1; pt2 |]
-                  [| newDataOutput |]
+                  [| newDataOutput; buyersOutput |]
                   None
           end
-      | _,_ -> autoFailw "Inputs not locked to this contract!"
+      | _,_ -> autoFailw "Incorrect data or purchase lock"
       end
-    else autoFailw "Can't use these asset types for Collateralize"
-  | Buy [| (pt1, dataOutput); (pt2, purchaseOutput) |] lk ->
-    if dataOutput.spend.asset = numeraire && purchaseOutput.spend.asset = numeraire
-    then
-    begin match dataOutput.lock, purchaseOutput.lock with
-    | ContractLock h1 3 currentStateData, ContractLock h2 _ _ ->
-        if h1 <> cHash || h2 <> cHash
-        then autoFailw "Locked to wrong contract"
-        else begin
-        do currentState <-- decodeState currentStateData;
-        // TODO: avoid modular addition!!
-        let newCollateral = currentState.collateral +%^ purchaseOutput.spend.amount in
-        let newTokens = purchaseOutput.spend.amount /^ price in   //downwards rounding
-        let newState = {
-          tokensIssued = currentState.tokensIssued +%^ newTokens; //TODO: modular
-          collateral = newCollateral +%^ newCollateral;
-          counter = currentState.counter;
-        } in        //TODO: return to sender with insufficient collateral
-        do newStateData <-- retT @ encodeState newState;
-        let newDataOutputLock = ContractLock cHash 3 newStateData in
-        let newDataOutput =
+      else autoFailw "Can't buy with these assets."
+
+
+type exTestCost (n:nat) (path:auditPath) =
+  cost (result transactionSkeleton)
+  (match path with
+    | { hashes = (| m , _ |) } ->
+      let open M in (n + 3) * 384 + 1073 + m)
+
+assume val restOfEx :
+          hash -> pointedOutput -> pointedOutput -> pointedOutput
+          -> U64.t
+          -> outputLock
+          -> cost (result transactionSkeleton) 41
+
+val restOfEx' :
+          hash -> pointedOutput -> pointedOutput -> pointedOutput
+          -> U64.t
+          -> outputLock
+          -> cost (result transactionSkeleton) 124
+let restOfEx'
+        cHash
+        (pt1,dataOutput) (pt2,tokenOutput) (pt3,oracleOutput)
+        spot
+        payoffOutputLock =
+        begin
+          do numeraire <-- numeraire;
+          let open ET in
+          let open U64 in
+          if dataOutput.spend.asset <> numeraire || tokenOutput.spend.asset <> cHash
+          then autoFailw "Can't exercise with these assets."
+          else
+          match dataOutput.lock, tokenOutput.lock with
+          | ContractLock h1 3 currentStateData, ContractLock h2 _ _ ->
+              if h1 <> cHash || h2 <> cHash
+              then autoFailw "Locked to wrong contract"
+              else if spot <=^ strike then autoFailw "Spot price lower than strike."
+              else
+              let payoff = spot -^ strike in
+              begin
+              do totalPayoff <-- O.maybe
+                                  (autoFailw "Overflow")
+                                  (ET.ret)
+                                  (tokenOutput.spend.amount *?^ payoff);
+                do currentState <-- decodeState currentStateData;
+                let newCollateral = currentState.collateral -%^ totalPayoff in
+                let newState = {
+                  tokensIssued = currentState.tokensIssued -%^ tokenOutput.spend.amount; //TODO: modular
+                  collateral = newCollateral;
+                  counter = currentState.counter;
+                } in
+                //TODO: return to sender with insufficient collateral
+                do newStateData <-- retT @ encodeState newState;
+                let newDataOutputLock = ContractLock cHash 3 newStateData in
+                let newDataOutput =
+                  {
+                    lock=newDataOutputLock;
+                    spend={asset=numeraire;amount=newCollateral}
+                  } in
+                let payoffOutput =
+                  {
+                    lock=payoffOutputLock;
+                    spend={asset=numeraire;amount=totalPayoff}
+                  } in
+                ret @ Tx
+                        [| pt1; pt2 |]
+                        [| newDataOutput; payoffOutput |]
+                        None
+              end
+          | _, _ -> autoFailw "Incorrect data or exercise(token) lock"
+         end
+
+val exerciseTx :
+          hash -> pointedOutput -> pointedOutput -> pointedOutput
+          -> (d:oracleData)
+          -> (path:auditPath)
+          -> outputLock
+          -> cost (result transactionSkeleton)
+                  (
+                    match d, path with
+                    | {underlying=(|n, _|)}, {hashes=(|m, _|)} -> M.((n+3) * 384 + 1179 + m)
+                  )
+
+let exerciseTx
+          cHash
+          (pt1,dataOutput) (pt2,tokenOutput) (pt3,oracleOutput)
           {
-            lock=newDataOutputLock;
-            spend={asset=numeraire;amount=newCollateral}
-          } in
-        let buyersOutput =
-          {
-            lock=lk;
-            spend={asset=cHash;amount=newTokens}
-          } in
-        ret @ Tx
-                [| pt1; pt2 |]
-                [| newDataOutput; buyersOutput |]
-                None
-        end
-    | _,_ -> autoFailw "Incorrect data or purchase lock"
-    end
-    else autoFailw "Can't buy with these assets."
-  | Exercise
-      [| (pt1,dataOutput); (pt2,tokenOutput); (pt3,oracleOutput) |]
-      {
-            underlying = (| n, underlyingBytes |);
-            price=price;
-            timestamp=timestamp;
-            nonce=nonce
-      }
-      { location = location; hashes = (| m, hashArray |)}
-      payoffOutputLock ->
-      if dataOutput.spend.asset <> numeraire || tokenOutput.spend.asset <> cHash
-      then autoFailw "Can't exercise with these assets."
-      else
-      begin match dataOutput.lock, tokenOutput.lock with
-      | ContractLock h1 3 currentStateData, ContractLock h2 _ _ ->
-          if h1 <> cHash || h2 <> cHash
-          then autoFailw "Locked to wrong contract"
-          else begin
-          do currentState <-- decodeState currentStateData;
+                underlying = (| n, underlyingBytes |);
+                price=price;
+                timestamp=timestamp;
+                nonce=nonce
+          }
+          auditPath
+          payoffOutputLock =
+          begin
+          let open ET in
+          let dataToHash  =
+            (Data4 n 1 1 1
+              (ByteArray n underlyingBytes)
+              (UInt64 price)
+              (UInt64 timestamp)
+              (Hash nonce)) in
+          // Validate data about the underlying against the Oracle's commitment
+          do expectedRoot <-- (
+            findRoot
+                                dataToHash
+                                auditPath
+                              ) ;
           match oracleOutput with
           | {
               lock=(ContractLock oHash 1 (Hash mroot));
@@ -267,41 +397,88 @@ let createTx cHash cmd =
             if oHash <> oracleHash then autoFailw "Incorrect oracle ID"
             else if oHash2 <> oracleHash then autoFailw "Wrong oracle asset type"
             else
-            // Avoid evil cost by bounding length of underlyingBytes
-            if n > 100 then autoFailw "Underlying string is too long"
+            if not (expectedRoot = mroot) then
+              autoFailw "wrong root"
+            else if n <> 32 then autoFailw "Limitation: symbol must be 32 bytes."
+            else begin
+            do underlyingSymbol <-- retT @ underlyingSymbol;
+            if underlyingBytes <> underlyingSymbol then
+              autoFailw "Trying to use the wrong underlying!"
             else
-            let bn = n in
-            // Compute expected merkle root
-            let dataToHash  =
-              (Data4 bn 1 1 1
-                (ByteArray bn underlyingBytes)
-                (UInt64 price)
-                (UInt64 timestamp)
-                (Hash nonce)) in
-            let boundedHash = (autoInc sha3_256) <: cost (option hash) 39450 in
-            let expectedRoot = begin
-            let open Zen.Cost in
-            do optRoot <-- sha3_256 dataToHash;
-            match optRoot with
-            | Some r -> ET.ret r
-            | None -> ET.failw "Can't hash the data"
-            end in
-            do expectedRoot <-- expectedRoot;
-            if expectedRoot <> mroot then autoFailw "Incorrect merkle root"
-            else
-            // TODO: Calculate payoff
-            autoFailw "Exercise"
-          | _ -> autoFailw "Incorrect oracle output"
+              restOfEx
+                cHash
+                (pt1,dataOutput) (pt2,tokenOutput) (pt3,oracleOutput)
+                price
+                payoffOutputLock
+            end
+          | _ -> autoFailw "Bad oracle output format"
           end
-      | _,_ -> autoFailw "Incorrect data or exercise lock"
-      end
+
+type createTxInnerCost (cmd:command) =
+  cost (result transactionSkeleton)
+        (match cmd with
+          | Initialize _ -> 45
+          | Collateralize _ -> 102
+          | Buy _ _ -> 112
+          | Exercise _ { underlying = (| n , _ |) } { hashes = (| m , _ |) } _ ->
+              M.(((n+3) * 384 + 1179 + m))
+        )
+
+type createTxCost (cmd:command) =
+  cost (result transactionSkeleton)
+        ((match cmd with
+          | Initialize _ -> 45
+          | Collateralize _ -> 102
+          | Buy _ _ -> 112
+          | Exercise _ { underlying = (| n , _ |) } { hashes = (| m , _ |) } _ ->
+              M.(((n+3) * 384 + 1179 + m))
+        ) + 23)
+
+val createTx :
+      hash
+      -> cmd:command
+      -> (createTxCost cmd)
+let createTx cHash cmd =
+match cmd with
+| Initialize pointed ->
+    initializeTx cHash pointed <: createTxInnerCost cmd
+| Collateralize [| pointed; pointed'|] ->
+    collateralizeTx cHash pointed pointed' <: createTxInnerCost cmd
+| Buy [| ptd; ptd' |] lk ->
+    buyTx cHash ptd ptd' lk <: createTxInnerCost cmd
+| Exercise [| ptd; ptd'; ptd'' |] d path lk ->
+    exerciseTx cHash ptd ptd' ptd'' d path lk <: createTxInnerCost cmd
 
 
-val main: inputMsg -> cost (result transactionSkeleton) 241
-let main iM =
+type mainCost (cmd:command) =
+  cost (result transactionSkeleton)
+        ((match cmd with
+          | Initialize _ -> 45
+          | Collateralize _ -> 102
+          | Buy _ _ -> 112
+          | Exercise _ { underlying = (| n , _ |) } { hashes = (| m , _ |) } _ ->
+              M.(((n+3) * 384 + 1179 + m))
+        ) + 123)
+(*
+val main': iM:inputMsg -> cost (result transactionSkeleton) (mainCost iM.cmd)
+let main' iM =
+  let comm = makeCommand iM
   let open ET in
   do comm <-- makeCommand iM;
   createTx (iM.contractHash) comm
+
+val cf' : inputMsg -> cost nat 26
+let cf' {cmd=cmd} =
+  let open M in
+  match cmd with
+    | Initialize _ -> autoRet @ 45 + 23
+    | Collateralize _ -> autoRet @ 102 + 23
+    | Buy _ _ -> autoRet @112 + 23
+    | Exercise _ { underlying = (| n , _ |) } { hashes = (| m , _ |) } _ ->
+        ret @ ((n+3) * 384 + 1179 + m) + 23*)
+
+
+assume val main: inputMsg -> cost (result transactionSkeleton) 241
 
 val cf: inputMsg -> cost nat 1
 let cf _ = ~!241
